processor/src/KamiProc.v
@@ -18,9 +18,10 @@ Section Parametrized.
             (exec: AbsExec iaddrSize instBytes dataBytes rfIdx)
             (ammio: AbsMMIO addrSize).
 
-  Variable (init: ProcInit iaddrSize dataBytes rfIdx).
+  Variable (procInit: ProcInit iaddrSize dataBytes rfIdx)
+           (memInit: MemInit addrSize dataBytes).
 
-  Definition pprocInl := scmmInl fetch dec exec ammio init.
+  Definition pprocInl := scmmInl fetch dec exec ammio procInit memInit.
   Definition pproc := projT1 pprocInl.
 
   (** The auxiliary hardware state; this is for manipulating hardware state
@@ -97,13 +98,191 @@ Section Parametrized.
       assumption.
   Qed.
 
+  Lemma invert_Kami_execLd_mmio:
+    forall km1 kt1 kupd klbl,
+      pRegsToT km1 = Some kt1 ->
+      Step pproc km1 kupd klbl ->
+      klbl.(annot) = Some (Some "execLd"%string) ->
+      exists curInst ldAddr,
+        curInst = (pgm kt1) (split2 _ _ (pc kt1)) /\
+        ldAddr = evalExpr
+                   (calcLdAddr
+                      _ (evalExpr (getLdAddr _ curInst))
+                      (rf kt1 (evalExpr (getLdSrc _ curInst)))) /\
+        (evalExpr (isMMIO _ ldAddr) = true ->
+         exists kt2 mmioLdRq mmioLdRs,
+           klbl.(calls) =
+           FMap.M.add
+             "mmioExec"%string
+             (existT SignT {| arg := Struct (RqFromProc addrSize dataBytes);
+                              ret := Struct (RsToProc dataBytes) |}
+                     (mmioLdRq, mmioLdRs))
+             (FMap.M.empty _) /\
+           mmioLdRq Fin.F1 = ldAddr /\
+           mmioLdRq (Fin.FS Fin.F1) = false /\
+           pRegsToT (FMap.M.union kupd km1) = Some kt2 /\
+           kt2 = {| pc := evalExpr (getNextPc _ (rf kt1) (pc kt1) curInst);
+                    rf :=
+                      fun w =>
+                        if weq w (evalExpr (getLdDst _ curInst))
+                        then mmioLdRs Fin.F1
+                        else rf kt1 w;
+                    pgm := pgm kt1;
+                    mem := mem kt1 |}).
+  Proof.
+    intros.
+    kinvert_more.
+    do 2 eexists; repeat split.
+    kinv_action_dest.
+    - unfold pRegsToT in *.
+      kregmap_red.
+      destruct (FMap.M.find "mem"%string km1) as [[[memk|] memv]|]; try discriminate.
+      destruct (decKind memk _); try discriminate.
+      kregmap_red.
+      inversion H; subst; clear H.
+      simpl in *.
+      repeat esplit.
+      + FMap.mred; eassumption.
+      + reflexivity.
+      + reflexivity.
+    - kinv_red.
+      unfold pRegsToT in *.
+      kregmap_red.
+      inversion H; subst; clear H; simpl in *.
+      exfalso; clear -H3 Heqic; congruence.
+  Qed.
+
+  Lemma invert_Kami_execLdZ:
+    forall km1 kt1 kupd klbl,
+      pRegsToT km1 = Some kt1 ->
+      Step pproc km1 kupd klbl ->
+      klbl.(annot) = Some (Some "execLdZ"%string) ->
+      klbl.(calls) = FMap.M.empty _ /\
+      exists kt2,
+        pRegsToT (FMap.M.union kupd km1) = Some kt2 /\
+        exists curInst,
+          curInst = (pgm kt1) (split2 _ _ (pc kt1)) /\
+          kt2 = {| pc := evalExpr (getNextPc _ (rf kt1) (pc kt1) curInst);
+                   rf := rf kt1;
+                   pgm := pgm kt1;
+                   mem := mem kt1 |}.
+  Proof.
+    intros.
+    kinvert_more.
+    kinv_action_dest.
+    unfold pRegsToT in *.
+    kregmap_red.
+    destruct (FMap.M.find "mem"%string km1) as [[[memk|] memv]|]; try discriminate.
+    destruct (decKind memk _); try discriminate.
+    kregmap_red.
+    inversion H; subst; clear H.
+    repeat esplit.
+    assumption.
+  Qed.
+
+  Lemma invert_Kami_execSt_memory:
+    forall km1 kt1 kupd klbl,
+      pRegsToT km1 = Some kt1 ->
+      Step pproc km1 kupd klbl ->
+      klbl.(annot) = Some (Some "execSt"%string) ->
+      exists curInst stAddr stVal,
+        curInst = (pgm kt1) (split2 _ _ (pc kt1)) /\
+        stAddr = evalExpr
+                   (calcStAddr
+                      _ (evalExpr (getStAddr _ curInst))
+                      (rf kt1 (evalExpr (getStSrc _ curInst)))) /\
+        stVal = rf kt1 (evalExpr (getStVSrc _ curInst)) /\
+        (evalExpr (isMMIO _ stAddr) = false ->
+         exists kt2,
+           klbl.(calls) = FMap.M.empty _ /\
+           pRegsToT (FMap.M.union kupd km1) = Some kt2 /\
+           kt2 = {| pc := evalExpr (getNextPc _ (rf kt1) (pc kt1) curInst);
+                    rf := rf kt1;
+                    pgm := pgm kt1;
+                    mem :=
+                      fun w =>
+                        if weq w stAddr then stVal else mem kt1 w |}).
+  Proof.
+    intros.
+    kinvert_more.
+    do 3 eexists; repeat split.
+    kinv_action_dest.
+    - unfold pRegsToT in *.
+      kregmap_red.
+      destruct (FMap.M.find "mem"%string km1) as [[[memk|] memv]|]; try discriminate.
+      destruct (decKind memk _); try discriminate.
+      kregmap_red.
+      inversion H; subst; clear H.
+      simpl in *.
+      exfalso; clear -H3 Heqic; congruence.
+    - kinv_red.
+      unfold pRegsToT in *.
+      kregmap_red.
+      inversion H; subst; clear H; simpl in *.
+      repeat esplit.
+      assumption.
+  Qed.
+
+  Lemma invert_Kami_execSt_mmio:
+    forall km1 kt1 kupd klbl,
+      pRegsToT km1 = Some kt1 ->
+      Step pproc km1 kupd klbl ->
+      klbl.(annot) = Some (Some "execSt"%string) ->
+      exists curInst stAddr stVal,
+        curInst = (pgm kt1) (split2 _ _ (pc kt1)) /\
+        stAddr = evalExpr
+                   (calcStAddr
+                      _ (evalExpr (getStAddr _ curInst))
+                      (rf kt1 (evalExpr (getStSrc _ curInst)))) /\
+        stVal = rf kt1 (evalExpr (getStVSrc _ curInst)) /\
+        (evalExpr (isMMIO _ stAddr) = true ->
+         exists kt2 mmioStRq mmioStRs,
+           klbl.(calls) =
+           FMap.M.add
+             "mmioExec"%string
+             (existT SignT {| arg := Struct (RqFromProc addrSize dataBytes);
+                              ret := Struct (RsToProc dataBytes) |}
+                     (mmioStRq, mmioStRs))
+             (FMap.M.empty _) /\
+           mmioStRq Fin.F1 = stAddr /\
+           mmioStRq (Fin.FS Fin.F1) = true /\
+           mmioStRq (Fin.FS (Fin.FS Fin.F1)) = stVal /\
+           pRegsToT (FMap.M.union kupd km1) = Some kt2 /\
+           kt2 = {| pc := evalExpr (getNextPc _ (rf kt1) (pc kt1) curInst);
+                    rf := rf kt1;
+                    pgm := pgm kt1;
+                    mem := mem kt1 |}).
+  Proof.
+    intros.
+    kinvert_more.
+    do 3 eexists; repeat split.
+    kinv_action_dest.
+    - unfold pRegsToT in *.
+      kregmap_red.
+      destruct (FMap.M.find "mem"%string km1) as [[[memk|] memv]|]; try discriminate.
+      destruct (decKind memk _); try discriminate.
+      kregmap_red.
+      inversion H; subst; clear H.
+      simpl in *.
+      repeat esplit.
+      + FMap.mred; eassumption.
+      + reflexivity.
+      + reflexivity.
+      + reflexivity.
+    - kinv_red.
+      unfold pRegsToT in *.
+      kregmap_red.
+      inversion H; subst; clear H; simpl in *.
+      exfalso; clear -H3 Heqic; congruence.
+  Qed.
+
   Lemma invert_Kami_execNm:
     forall km1 kt1 kupd klbl,
       pRegsToT km1 = Some kt1 ->
       Step pproc km1 kupd klbl ->
       klbl.(annot) = Some (Some "execNm"%string) ->
+      klbl.(calls) = FMap.M.empty _ /\
       exists kt2,
-        klbl.(calls) = FMap.M.empty _ /\
         pRegsToT (FMap.M.union kupd km1) = Some kt2 /\
         exists curInst execVal,
           curInst = (pgm kt1) (split2 _ _ (pc kt1)) /\
@@ -151,12 +330,13 @@ Section PerInstAddr.
   Definition procInit: ProcInit ninstrMemSizeLg rv32DataBytes rv32RfIdx :=
     {| pcInit := getDefaultConst _;
        rfInit := getDefaultConst _ |}.
+  Variable (memInit: MemInit nwidth rv32DataBytes).
 
   Definition predictNextPc ty (ppc: fullType ty (SyntaxKind (Pc ninstrMemSizeLg))) :=
     (#ppc + $4)%kami_expr.
 
   Definition procInl :=
-    pprocInl rv32Fetch (rv32Dec _) (rv32Exec _) rv32MMIO procInit.
+    pprocInl rv32Fetch (rv32Dec _) (rv32Exec _) rv32MMIO procInit memInit.
   Definition proc: Kami.Syntax.Modules := projT1 procInl.
 
   Definition hst := Kami.Semantics.RegsT.
@@ -171,7 +351,8 @@ Section PerInstAddr.
   (** Refinement from [p4mm] to [proc] (as a spec) *)
 
   Definition p4mm: Kami.Syntax.Modules :=
-    p4mm 1 rv32Fetch (rv32Dec _) (rv32Exec _) rv32MMIO predictNextPc procInit.
+    p4mm 1 rv32Fetch (rv32Dec _) (rv32Exec _) rv32MMIO
+         predictNextPc procInit memInit.
 
   Theorem proc_correct: p4mm <<== proc.
   Proof.
